Axioms in certicoq:
So far I have added a new Term constructor (TAx : Term -> Term).  The
argument to TAx is the axiom's type, so this is like having a single
undefined value shared by all axioms.  The various evaluators simply
block on this constant.

I've carried this approach through all of L1, L2 and L3.  This should
evaluate the same as Coq.  On Abishek's example

    Axiom feq1 : (fun x:nat => x) = (fun x:nat => x+x-x).

(with fuel-driven weak cbv evaluation) in L1, L2, and L3, the current
version does indeed agree with Coq.

NOTE: My tests (test_wcbvEval.v in directories L1, L2 and L3) compare

- quoting and translation to Ln followed by evaluation in Ln, 
- evaluation (in Coq) followed by quoting and and translation to Ln.

Once a test rig is set up for each language (a few lines of Coq),
examples are tested with [vm_compute; reflexivity].

If we allow axioms to not block evaluation (e.g. if every match with
only one branch always steps), then this easy testing no longer works.

"make"ing the whole project now fails on

File "./L4_deBruijn/L3_to_L4.v", line 46, characters 2-1365:
Error: Non exhaustive pattern-matching: ...

Since L4 doesn't yet have a TAx term constructor.

theories/L1_MalechaQuoted/term.v
@@ -12,9 +12,11 @@ Local Open Scope list.
 Set Implicit Arguments.
 
 (** A slightly cleaned up notion of object term.
-*** The simultaneous definitions of [Terms] and [Defs] make inductions
-*** proof over this type long-winded but straightforward
+*** The simultaneous definitions of [Terms] and [Defs] make
+*** inductions over this type long-winded but straightforward.
 *** This version contains type fields.
+*** There is a special term constructor for axioms, which
+*** should be seen as having a type but no value.
 **)
 Inductive Term : Type :=
 | TRel       : nat -> Term
@@ -31,6 +33,7 @@ Inductive Term : Type :=
 | TCase      : (nat * list nat) (* # of parameters, args per branch *) ->
                Term (* type info *) -> Term -> Terms -> Term
 | TFix       : Defs -> nat -> Term
+| TAx        : Term -> Term (* type *)
 with Terms : Type :=
 | tnil : Terms
 | tcons : Term -> Terms -> Terms
@@ -50,44 +53,6 @@ Notation prop := (TSort SProp).
 Notation set_ := (TSort SSet).
 Notation type_ := (TSort SType).
 Notation tunit t := (tcons t tnil).
-
-Definition TrmTrmsDefs_Typeind 
-  (P : Term -> Type) (P0 : Terms -> Type) (P1 : Defs -> Type)
-  (f : forall n : nat, P (TRel n)) (f0 : forall s : Srt, P (TSort s))
-  (f1 : forall t : Term,
-        P t -> forall (c : cast_kind) (t0 : Term), P t0 -> P (TCast t c t0))
-  (f2 : forall (n : name) (t : Term),
-        P t -> forall t0 : Term, P t0 -> P (TProd n t t0))
-  (f3 : forall (n : name) (t : Term),
-        P t -> forall t0 : Term, P t0 -> P (TLambda n t t0))
-  (f4 : forall (n : name) (t : Term),
-        P t ->
-        forall t0 : Term,
-        P t0 -> forall t1 : Term, P t1 -> P (TLetIn n t t0 t1))
-  (f5 : forall t : Term,
-        P t ->
-        forall t0 : Term,
-        P t0 -> forall t1 : Terms, P0 t1 -> P (TApp t t0 t1))
-  (f6 : forall s : string, P (TConst s))
-  (f7 : forall i : inductive, P (TInd i))
-  (f8 : forall (i : inductive) (n : nat), P (TConstruct i n))
-  (f9 : forall (n : nat * list nat) (t : Term),
-        P t ->
-        forall t0 : Term,
-        P t0 -> forall t1 : Terms, P0 t1 -> P (TCase n t t0 t1))
-  (f10 : forall d : Defs, P1 d -> forall n : nat, P (TFix d n))
-  (f11 : P0 tnil)
-  (f12 : forall t : Term, P t -> forall t0 : Terms, P0 t0 -> P0 (tcons t t0))
-  (f13 : P1 dnil)
-  (f14 : forall (n : name) (t : Term),
-         P t ->
-         forall t0 : Term,
-         P t0 -> forall (n0 : nat) (d : Defs), P1 d -> P1 (dcons n t t0 n0 d))
-  : (forall t : Term, P t) * (forall t : Terms, P0 t) * (forall d : Defs, P1 d)
-  := (pair
-     (pair (Trm_ind2 P P0 P1 f f0 f1 f2 f3 f4 f5 f6 f7 f8 f9 f10 f11 f12 f13 f14)
-     (Trms_ind2 P P0 P1 f f0 f1 f2 f3 f4 f5 f6 f7 f8 f9 f10 f11 f12 f13 f14))
-     (Defs_ind2 P P0 P1 f f0 f1 f2 f3 f4 f5 f6 f7 f8 f9 f10 f11 f12 f13 f14)).
 
 
 Section TermTerms_dec. (** to make Ltac definitions local **)
@@ -127,6 +92,7 @@ apply TrmTrmsDefs_ind.
   destruct (H1 t2); [lft | rght .. ].
 - induction t; cross.
   destruct (eq_nat_dec n n0); destruct (H d0); [lft | rght .. ].
+- induction t0; cross. destruct (H t0); [lft | rght ..].
 - induction tt; cross. lft.
 - induction tt; cross. destruct (H t1); destruct (H0 tt); [lft | rght .. ].
 - induction ee; cross. lft.
@@ -672,6 +638,8 @@ Proof.
   left. intuition. revert H. not_isApp.
 - exists (TFix d n), arg, tnil. split. reflexivity.
   left. intuition. revert H. not_isApp.
+- exists (TAx fn), arg, tnil. split. reflexivity.
+  left. intuition. revert H. not_isApp.
 Qed.
 
 (** well-formed terms: TApp well-formed all the way down **)
@@ -696,6 +664,7 @@ Inductive WFapp: Term -> Prop :=
             WFapp mch -> WFapps brs -> WFapp ty ->
             WFapp (TCase m ty mch brs)
 | wfaFix: forall defs m, WFappDs defs -> WFapp (TFix defs m)
+| wfaAx: forall ty, WFapp ty -> WFapp (TAx ty)
 with WFapps: Terms -> Prop :=
 | wfanil: WFapps tnil
 | wfacons: forall t ts, WFapp t -> WFapps ts -> WFapps (tcons t ts)
@@ -818,6 +787,7 @@ Inductive WFTrm: Term -> nat -> Prop :=
             WFTrm (TCase m ty mch brs) n
 | wfFix: forall n defs m,
            WFTrmDs defs (n + dlength defs) -> WFTrm (TFix defs m) n
+| wfAx: forall n ty, WFTrm ty n -> WFTrm (TAx ty) n
 with WFTrms: Terms -> nat -> Prop :=
 | wfnil: forall n, WFTrms tnil n
 | wfcons: forall n t ts, WFTrm t n -> WFTrms ts n -> WFTrms (tcons t ts) n
@@ -868,6 +838,7 @@ Inductive PoccTrm : Term -> Prop :=
 | PoCaseR: forall n ty mch brs, PoccTrms brs -> PoccTrm (TCase n ty mch brs)
 | PoCaseTy: forall n ty mch brs, PoccTrm ty -> PoccTrm (TCase n ty mch brs)
 | PoFix: forall ds m, PoccDefs ds -> PoccTrm (TFix ds m)
+| PoAx: forall ty, PoccTrm ty -> PoccTrm (TAx ty)
 | PoCnstr: forall m1 m2, PoccTrm (TConstruct (mkInd nm m1) m2)
 with PoccTrms : Terms -> Prop :=
 | PoThd: forall t ts, PoccTrm t -> PoccTrms (tcons t ts)
@@ -1119,6 +1090,9 @@ Proof.
     + apply PoFix. assumption.
     + apply PoAppL. apply PoFix. assumption.
   - destruct args; simpl.
+    + apply PoAx. assumption.
+    + apply PoAppL. apply PoAx. assumption.
+  - destruct args; simpl.
     + apply PoCnstr; assumption.
     + apply PoAppL. apply PoCnstr.
 Qed.
@@ -1183,6 +1157,8 @@ Inductive Instantiate: nat -> Term -> Term -> Prop :=
 | IFix: forall n d m id, 
           InstantiateDefs (n + dlength d) d id ->
           Instantiate n (TFix d m) (TFix id m)
+| IAx: forall n ty ity,
+         Instantiate n ty ity -> Instantiate n (TAx ty) (TAx ity)
 with Instantiates: nat -> Terms -> Terms -> Prop :=
 | Inil: forall n, Instantiates n tnil tnil
 | Icons: forall n t ts it its,
@@ -1241,6 +1217,7 @@ intro h. apply InstInstsDefs_ind; intros; auto.
   + apply PoCaseTy. apply H0. assumption.
 - inversion_Clear H0.
   + constructor. apply H. assumption.
+- inversion_Clear H0. constructor. intuition.
 - inversion_Clear H1.
   + constructor. apply H. assumption.
   + apply PoTtl. apply H0. assumption.
@@ -1267,6 +1244,7 @@ Function instantiate (n:nat) (tbod:Term) {struct tbod} : Term :=
     | TLetIn nm tdef ty bod =>
       TLetIn nm (instantiate n tdef) (instantiate n ty) (instantiate (S n) bod)
     | TFix ds m => TFix (instantiateDefs (n + dlength ds) ds) m
+    | TAx ty => TAx (instantiate n ty)
     | TCast t ck ty => TCast (instantiate n t) ck (instantiate n ty)
     | x => x
   end
@@ -1321,6 +1299,7 @@ apply TrmTrmsDefs_ind; intros; simpl; try (solve [constructor]).
 - apply IApp; intuition.
 - apply ICase; intuition.
 - apply IFix; intuition.
+- apply IAx. intuition.
 - apply Icons; intuition.
 - apply Idcons; intuition.
 Qed.
@@ -1401,6 +1380,8 @@ Proof.
    - change (WFapp (TFix (instantiateDefs t (n + dlength defs) defs) m)).
      constructor.
      + apply H0. assumption.
+   - change (WFapp (TAx (instantiate t n ty))).
+     constructor. apply H0. assumption.
    - change (WFapps (tcons (instantiate t0 n t) (instantiates t0 n ts))).
      constructor.
      + apply H0. assumption.
