theories/L3_flattenedApp/program.v
@@ -1,5 +1,4 @@
 
-
 Require Import Lists.List.
 Require Import Strings.String.
 Require Import Strings.Ascii.
@@ -292,6 +291,7 @@ Inductive Crct: environ -> nat -> Term -> Prop :=
 | CrctFix: forall n p ds m,
              Crct p n prop ->    (** convenient for IH *)
              CrctDs p (n + dlength ds) ds -> Crct p n (TFix ds m)
+| CrctAx: forall n p ty, Crct p n ty -> Crct p n (TAx ty)
 | CrctInd: forall n p ind, Crct p n prop -> Crct p n (TInd ind)
 with Crcts: environ -> nat -> Terms -> Prop :=
 | CrctsNil: forall n p, Crct p n prop -> Crcts p n tnil
@@ -344,6 +344,7 @@ apply CrctCrctsCrctDsTyp_ind; intros.
 - eapply CrctConstruct; eassumption.
 - apply CrctCase; assumption.
 - apply CrctFix; assumption.
+- apply CrctAx; assumption.
 - apply CrctInd; assumption.
 - apply CrctsNil; assumption.
 - apply CrctsCons; assumption.
@@ -552,6 +553,8 @@ apply CrctCrctsCrctDsTyp_ind; intros; auto.
 - apply CrctFix.
   + eapply H0. eassumption. intros h. inversion h.
   + eapply H2. eassumption. intros h. elim H4. apply PoFix. assumption.
+- apply CrctAx. apply (H0 _ _ _ H1). intros h. elim H2.
+  apply PoAx. assumption.        
 - apply CrctInd. apply (H0 _ _ _ H1). inversion 1. 
 - apply CrctsNil. rewrite H1 in H. inversion H; assumption.
 - apply CrctsCons.
@@ -718,6 +721,15 @@ induction 1; intros; try discriminate.
 - injection H1; intros; subst. assumption.
 Qed.
 
+Lemma Crct_invrt_Ax:
+  forall p n t, Crct p n t ->
+  forall u, t = (TAx u) -> Crct p n u.
+induction 1; intros; try discriminate.
+- apply (proj1 Crct_weaken); intuition.
+- specialize (IHCrct _ H2). apply (proj1 Crct_Typ_weaken); intuition.
+- myInjection H0. assumption.
+Qed.
+
 Lemma Crct_invrt_Construct:
   forall p n construct, Crct p n construct ->
   forall ipkgNm inum cnum args,
@@ -794,6 +806,8 @@ Proof.
       * simpl in j. generalize (dlength d). induction n0.
         rewrite <- plus_n_O. assumption.
         rewrite <- plus_n_Sm. apply (proj1 Crct_up). assumption.
+  - apply CrctAx. apply H; try assumption.
+    apply (Crct_invrt_Ax H1 eq_refl).
   - apply CrctsNil. eapply Crct_Sort. eassumption.
   - inversion_Clear H2. apply CrctsCons.
     + apply H; trivial.
